matching-logic/src/Theories/Sorts_ProofSystem.v
@@ -36,8 +36,16 @@ Open Scope list_scope.
 
 Set Printing All.
 
+Ltac solve_sfresh :=
+  (eapply not_elem_of_larger_impl_not_elem_of;
+  [|apply X_eq_fresh_impl_X_notin_free_svars; reflexivity];
+  simpl; clear; set_solver) +
+  by (unfold svar_is_fresh_in;
+  eapply svar_is_fresh_in_richer'; [|apply set_svar_fresh_is_fresh'];
+  clear; set_solver).
 
-(* (*  eq-elim.0 $e #Substitution ph2 ph4 ph0 x $.   => ph2 = ph4[ph0/x]
+
+(*  eq-elim.0 $e #Substitution ph2 ph4 ph0 x $.   => ph2 = ph4[ph0/x]
     eq-elim.1 $e #Substitution ph3 ph4 ph1 x $.   => ph3 = ph4[ph1/x]
     eq-elim $a |- ( \imp ( \eq ph0 ph1 ) ( \imp ph2 ph3 ) ) $.
                                                   => ph0 = ph1 -> ph2 -> ph3
@@ -45,12 +53,14 @@ Set Printing All.
 Lemma equality_elimination_basic 
   {Σ : Signature}
   {sy : Definedness_Syntax.Syntax}
-  Γ φ1 φ2 C x (xs : EVarSet) X i
+  Γ φ1 φ2 C (* x (xs : EVarSet) X i *)
   (HΓ : theory ⊆ Γ)
   (WF1 : well_formed φ1)
   (WF2 :  well_formed φ2)
   (WFC : PC_wf C)
-  (Hfree : {[ev_x; x]} ∪ free_evars φ1 ∪ free_evars φ2 ∪ free_evars (pcPattern C) ## xs)
+  (Hmu : pattern_kt_well_formed (pcPattern C))
+  (* (Hmu : bound_svar_is_banned_under_mus (pcPattern C) 0 0) *)
+(*   (Hfree : {[ev_x; x]} ∪ free_evars φ1 ∪ free_evars φ2 ∪ free_evars (pcPattern C) ## xs)
   (Hfree2 : x ∉ free_evars φ1 ∪ free_evars φ2 ∪ free_evars (pcPattern C))
   (* (Hfree3 : x ∉ free_svars ) *)
   (Henough : size xs >= maximal_exists_depth_to 0 (pcEvar C) (pcPattern C)):
@@ -58,71 +68,55 @@ Lemma equality_elimination_basic
   ProofInfoLe (ExGen := {[ev_x; x]} ∪ coGset.gset_to_coGset xs,
          SVSubst := {[X]},
          KT := false,
-         AKT := false) i ->
+         AKT := false) i -> *) :
   Γ ⊢i (φ1 =ml φ2) --->
     (emplace C φ1) ---> (emplace C φ2)
-  using i.
+  using AnyReasoning.
 Proof.
   destruct C as [y φ4]. cbn in *.
   assert (well_formed φ4) by wf_auto2. clear WFC.
   remember (size' φ4) as sz.
   assert (size' φ4 <= sz) by lia. clear Heqsz.
-  revert φ4 φ1 φ2 xs x X Γ HΓ H0 H WF1 WF2 Hfree Hfree2 Henough. induction sz; intros.
+  revert φ4 φ1 φ2 (* xs x X *) Γ HΓ H0 H WF1 WF2 Hmu (* Hfree Hfree2 Henough *). induction sz; intros.
   {
     destruct φ4; simpl in H0; lia.
   }
   destruct φ4; simpl in *.
   * case_match.
-    - subst. rewrite decide_eq_same.
+    - subst.
       mlIntro "H".
       (* ExGen : {[ev_x; x]} is needed for this: *)
       mlApplyMeta total_phi_impl_phi in "H".
       (***)
       mlDestructAnd "H".
       mlAssumption.
-      3: wf_auto2.
-      1: instantiate (1 := x).
-      try_solve_pile.
-      set_solver.
-    - rewrite decide_False. by auto.
-      rewrite decide_False. by auto.
-      do 2 mlIntro. mlAssumption.
+      2: assumption.
+      1: instantiate (1 := fresh_evar (φ1 ---> φ2)); solve_fresh.
+    - do 2 mlIntro. mlAssumption.
   * do 2 mlIntro. mlAssumption.
   * do 2 mlIntro. mlAssumption.
   * do 2 mlIntro. mlAssumption.
   * do 2 mlIntro. mlAssumption.
   * mlIntro "H".
-    epose proof (IH1 := IHsz φ4_1 φ1 φ2 xs x X Γ HΓ ltac:(lia) ltac:(wf_auto2) ltac:(wf_auto2) ltac:(wf_auto2) _ ltac:(set_solver) ltac:(lia) H1).
-    epose proof (IH2 := IHsz φ4_2 φ1 φ2 xs x X Γ HΓ ltac:(lia) ltac:(wf_auto2) ltac:(wf_auto2) ltac:(wf_auto2) _ ltac:(set_solver) ltac:(lia) H1).
+    epose proof (IH1 := IHsz φ4_1 φ1 φ2 (* xs x X *) Γ HΓ ltac:(lia) ltac:(wf_auto2) ltac:(wf_auto2) ltac:(wf_auto2) ltac:(by destruct_and!) (*_ ltac:(set_solver) ltac:(lia) H1 *)).
+    epose proof (IH2 := IHsz φ4_2 φ1 φ2 (* xs x X *) Γ HΓ ltac:(lia) ltac:(wf_auto2) ltac:(wf_auto2) ltac:(wf_auto2) ltac:(by destruct_and!) (* _ ltac:(set_solver) ltac:(lia) H1 *)).
     clear IHsz.
     mlAssert ("H2" : (φ1 =ml φ2)). wf_auto2. mlAssumption.
-    eapply framing_left_under_tot_impl with (x := x) in IH1.
-    eapply framing_right_under_tot_impl with (x := x) in IH2.
+    eapply framing_left_under_tot_impl with (x := fresh_evar ((φ1 <---> φ2) ---> φ4_2^[[evar:y↦φ2]])) in IH1.
+    eapply framing_right_under_tot_impl with (x := fresh_evar ((φ1 <---> φ2) ---> φ4_1^[[evar:y↦φ1]])) in IH2.
     mlApplyMeta IH1 in "H".
     mlApplyMeta IH2 in "H2".
     mlIntro "H0".
     mlApply "H".
     mlApply "H2".
     mlAssumption.
-    5, 12: assumption.
+    6, 13: solve_fresh.
     6, 12: try_solve_pile.
-    1-4,6-9: wf_auto2.
-    1-2: clear -Hfree2; pose proof free_evars_free_evar_subst; set_solver.
-    Unshelve.
-    - clear -Hfree.
-      apply disjoint_union_l in Hfree as [HF1 HF2].
-      apply disjoint_union_l in HF1 as [H ?], HF2 as [? ?].
-      apply disjoint_union_l in H as [? ?].
-      set_solver.
-    - clear -Hfree.
-      apply disjoint_union_l in Hfree as [HF1 HF2].
-      apply disjoint_union_l in HF1 as [H ?], HF2 as [? ?].
-      apply disjoint_union_l in H as [? ?].
-      set_solver.
+    all: try assumption; wf_auto2.
   * do 2 mlIntro. mlAssumption.
   * mlIntro "H".
-    epose proof (IH1 := IHsz φ4_1 φ2 φ1 xs x X Γ HΓ ltac:(lia) ltac:(wf_auto2) ltac:(wf_auto2) ltac:(wf_auto2) _ ltac:(set_solver) ltac:(lia) H1).
-    epose proof (IH2 := IHsz φ4_2 φ1 φ2 xs x X Γ HΓ ltac:(lia) ltac:(wf_auto2) ltac:(wf_auto2) ltac:(wf_auto2) _ ltac:(set_solver) ltac:(lia) H1).
+    epose proof (IH1 := IHsz φ4_1 φ2 φ1 (* xs x X *) Γ HΓ ltac:(lia) ltac:(wf_auto2) ltac:(wf_auto2) ltac:(wf_auto2) ltac:(by destruct_and!)(* _ ltac:(set_solver) ltac:(lia) H1 *)).
+    epose proof (IH2 := IHsz φ4_2 φ1 φ2 (* xs x X *) Γ HΓ ltac:(lia) ltac:(wf_auto2) ltac:(wf_auto2) ltac:(wf_auto2) ltac:(by destruct_and!)(* _ ltac:(set_solver) ltac:(lia) H1 *)).
     clear IHsz.
     mlAssert ("H2" : (φ2 =ml φ1)). wf_auto2.
     {
@@ -132,17 +126,6 @@ Proof.
     mlApplyMeta IH2 in "H".
     mlIntro "H0". mlIntro "S".
     clear. mlApply "H". mlApply "H0". mlApply "H2". mlAssumption.
-    Unshelve.
-    - clear -Hfree.
-      apply disjoint_union_l in Hfree as [HF1 HF2].
-      apply disjoint_union_l in HF1 as [H ?], HF2 as [? ?].
-      apply disjoint_union_l in H as [? ?].
-      set_solver.
-    - clear -Hfree.
-      apply disjoint_union_l in Hfree as [HF1 HF2].
-      apply disjoint_union_l in HF1 as [H ?], HF2 as [? ?].
-      apply disjoint_union_l in H as [? ?].
-      set_solver.
   * mlIntro.
     mlIntro.
     destruct (decide (y ∈ free_evars φ4)).
@@ -151,147 +134,112 @@ Proof.
       rewrite free_evar_subst_no_occurrence. assumption.
       mlAssumption.
     }
-    rewrite maximal_exists_depth_to_S in Henough. assumption.
-    destruct (elements xs) eqn:Hel.
-    {
-      apply elements_empty_iff in Hel. apply leibniz_equiv in Hel.
-      subst. rewrite size_empty in Henough. lia.
-    }
-    rename e0 into z.
-    (* TODO: extract this, very technical *)
-    assert (xs = {[z]} ∪ list_to_set l). {
-      rewrite <- (list_to_set_cons z l).
-      clear-Hel.
-      rewrite <- list_to_set_elements_L at 1.
-      by rewrite Hel.
-    }
-    assert (z ∉ l /\ z <> y) as HZ. {
-      split.
-      pose proof (HND := NoDup_elements xs).
-      clear -Hel HND.
-      rewrite Hel in HND. inversion HND. set_solver.
-      set_solver.
-    }
-    subst xs.
-    assert (z ∉ free_evars φ1 ∪ free_evars φ2 ∪ free_evars φ4). {
-      clear-Hfree. apply disjoint_union_r in Hfree. set_solver.
-    }
+
     (* TODO
        manually applied mlDestructEx, because it does not automatically solve the
        side conditions, thus fails *)
+    mlFreshEvar as z.
     _mlReshapeHypsByName "1".
-    apply MLGoal_destructEx with (x := z). try_solve_pile.
-    1-4: cbn; clear-H2.
-    1-2: set_solver.
-    1-2: pose proof free_evars_free_evar_subst; set_solver.
+    eapply MLGoal_destructEx with z. apply pile_any.
+
+    1: ltac2:(_fm_export_everything()); cbn; set_solver.
+    1: ltac2:(_fm_export_everything()); cbn; set_solver.
+    1: ltac2:(_fm_export_everything()); cbn; pose proof free_evars_free_evar_subst; set_solver.
+    1: ltac2:(_fm_export_everything()); cbn; pose proof free_evars_free_evar_subst; set_solver.
     (* *** *)
     simpl. mlExists z.
-    opose proof* (IHsz (evar_open z 0 φ4) φ1 φ2 (list_to_set l) x X Γ HΓ).
+    opose proof* (IHsz (evar_open z 0 φ4) φ1 φ2 (* (list_to_set l) x X *) Γ HΓ).
     2-4: wf_auto2.
     1: rewrite evar_open_size'; lia.
-    - clear -Hfree e HZ.
-      pose proof free_evars_evar_open φ4 z 0.
-      repeat apply disjoint_union_r in Hfree as [Hfree ?].
-      repeat apply disjoint_union_l in Hfree as [Hfree ?].
-      repeat apply disjoint_union_l in H0 as [H0 ?].
-      repeat (apply disjoint_union_l; split); try assumption.
-      clear -H5 H HZ. set_solver.
-    - pose proof free_evars_evar_open φ4 z 0.
-      clear-Hfree2 Hfree H3.
-      repeat apply disjoint_union_r in Hfree as [Hfree _].
-      do 3 apply disjoint_union_l in Hfree as [Hfree _].
-      apply disjoint_union_l in Hfree as [_ Hfree].
-      set_solver.
-    - rewrite evar_open_exists_depth.
-      set_solver.
-      rewrite size_union in Henough. set_solver.
-      rewrite size_singleton in Henough. lia.
-    - try_solve_pile.
-    - rewrite evar_open_free_evar_subst_swap. apply HZ. wf_auto2.
-      rewrite evar_open_free_evar_subst_swap. apply HZ. wf_auto2.
-      mlApplyMeta H3. mlSplitAnd; mlAssumption.
+    1: by apply kt_well_formed_evar_open.
+    rewrite evar_open_free_evar_subst_swap. fm_solve. wf_auto2.
+    rewrite evar_open_free_evar_subst_swap. fm_solve. wf_auto2.
+    mlApplyMeta H1. mlSplitAnd; mlAssumption.
   * do 2 mlIntro.
-    epose proof (floor_is_predicate Γ (φ1 <---> φ2) i x _ _ HΓ
-                   ltac:(wf_auto2) ltac:(set_solver) _ _ _) as Hpred.
-    unfold is_predicate_pattern in Hpred.
-    mlAdd Hpred. mlDestructOr "2".
-    {
-      opose proof* (IHsz (svar_open X 0 φ4) φ1 φ2 xs x X Γ HΓ) as IHsz.
-      1-8: admit.
-      mlAdd IHsz.
-    }
-    {
-    
-    }
-    (* Search patt_or derives_using.
-    
-    assert (). *)
-    
-    (*
-      new idea:
-      1. prove Γ ⊢ is_predicate (φ = ψ) -> Γ ⊢ φ = ⊤ or φ = ⊥   (maybe with <--->)
-                                                                (maybe with meta-or)
-      2. do case separation based on 1.
-        a) if φ = ⊥, then contradiction
-        b) if φ = ⊤, then it can be eliminated from IHsz, also from the goal.
-           then use mu_monotone
-    *)
-  
-  
-    Search derives_using (_ ---> _ ---> _).
-    Check prf_equiv_congruence.
-    Search is_predicate_pattern derives_using.
-    opose proof* (IHsz (svar_open X 0 φ4) φ1 φ2 xs x X Γ HΓ) as IHsz.
-    1-8: admit.
-    pose proof (move_mu_under_implication Γ (φ1 =ml φ2) (φ4^[[evar:y↦φ1]])
+    mlConj "0" "1" as "H". mlClear "0". mlClear "1".
+    opose proof* (mu_and_predicate_propagation Γ (φ4^[[evar:y↦φ1]]) (φ1 =ml φ2) HΓ
       ltac:(wf_auto2) ltac:(wf_auto2)).
-    (** TODO ***)
-    replace (ExGen := ∅ : coEVarSet, SVSubst := ∅ : coSVarSet, KT := true,
-            AKT := ~~ bound_svar_is_banned_under_mus φ4^[[evar:y↦φ1]] 0 0) with
-      i in H2.
-    (****)
-    mlAssert ("H" : ((mu , φ1 =ml φ2 ---> φ4^[[evar:y↦φ1]]))). { admit. }
     {
-      mlApplyMeta H2. mlSplitAnd; mlAssumption.
+      destruct_and!.
+      apply bound_svar_is_banned_under_mus_fevar_subst_alternative.
+      * wf_auto2.
+      * apply bsvar_occur_false_impl_banned.
+        apply wfc_mu_aux_implies_not_bsvar_occur. wf_auto2.
+      * assumption.
     }
-    
-    mlApplyMeta H2 in "0".
-    mlApply "0" in "1".
-    mlClear "0".
-    mlClear "1".
-    fromMLGoal. clear H2.
-    replace ((mu , φ1 =ml φ2 ---> φ4^[[evar:y↦φ1]]) ---> (mu , φ4^[[evar:y↦φ2]]))
+    {
+      remember (fresh_evar (φ1 ---> φ2)) as x.
+      remember (fresh_evar (φ1 ---> φ2 ---> patt_free_evar x)) as z.
+      remember (fresh_evar (φ1 ---> φ2 ---> patt_free_evar x --->
+                patt_free_evar z)) as w.
+      eapply floor_is_predicate with (x := x) (y := z) (z := w); try eassumption.
+      wf_auto2.
+      1-3: subst; simpl; solve_fresh.
+      try_solve_pile.
+    }
+    apply pf_iff_proj2 in H1. 2-3: wf_auto2.
+    2-5: try apply wfc_impl_no_pos_occ; try apply wfc_impl_no_neg_occ; wf_auto2.
+    mlApplyMeta H1 in "H".
+    remember (fresh_svar (φ1 ---> φ2 ---> φ4 ---> patt_free_evar y)) as X.
+    fromMLGoal.
+    replace ((mu , φ1 =ml φ2 and φ4^[[evar:y↦φ1]]) ---> (mu , φ4^[[evar:y↦φ2]]))
       with
-      ((mu , (φ1 =ml φ2 ---> φ4^[[evar:y↦φ1]])^{svar:0↦X}^{{svar:X↦0}}) ---> (mu , φ4^[[evar:y↦φ2]]^{svar:0↦X}^{{svar:X↦0}})).
+      ((mu , (φ1 =ml φ2 and φ4^[[evar:y↦φ1]])^{svar:0↦X}^{{svar:X↦0}}) ---> (mu , φ4^[[evar:y↦φ2]]^{svar:0↦X}^{{svar:X↦0}})).
+    (* TODO: solve_sfresh seems to not work well here *)
     2: {
-      admit.
+      mlSimpl.
+      rewrite !svar_quantify_svar_open.
+      1-8: try wf_auto2.
+      1-2: solve_sfresh.
+      1-2: pose proof free_svars_free_evar_subst.
+      1-2: eapply not_elem_of_larger_impl_not_elem_of;
+  [|apply X_eq_fresh_impl_X_notin_free_svars; reflexivity];
+      cbn; set_solver.
+      reflexivity.
     }
-    apply mu_monotone.
-    - admit.
-    - apply svar_hno_bsvar_subst.
-      + intro HH. cbn in HH. congruence.
-      + intros. wf_auto2.
-        all: try apply wfc_impl_no_neg_occ; try apply wfc_impl_no_pos_occ.
-        all: wf_auto2.
-      + intros. apply fresh_svar_no_neg. admit.
-    - apply svar_hno_bsvar_subst.
-      + intro HH. cbn in HH. congruence.
-      + intros. wf_auto2.
-        all: try apply wfc_impl_no_neg_occ; try apply wfc_impl_no_pos_occ.
-        all: wf_auto2.
-      + intros. apply fresh_svar_no_neg. admit.
-    - mlSimpl.
-      rewrite (svar_open_not_occur 0 X φ1). wf_auto2.
-      rewrite (svar_open_not_occur 0 X φ2). wf_auto2.
-      unfold svar_open.
-      rewrite <- free_evar_subst_bsvar_subst.
-      rewrite <- free_evar_subst_bsvar_subst.
-      2,4:wf_auto2.
-      2-3: unfold evar_is_fresh_in; set_solver.
-      fold (svar_open X 0 φ4).
-      
-      apply IHsz.
-Defined. *)
+
+    aapply mu_monotone.
+    {
+      apply svar_hno_bsvar_subst.
+      * intros. cbn in H2. congruence.
+      * intros. clear-H WF1 WF2. wf_auto2.
+        all: try apply wfc_impl_no_pos_occ; try apply wfc_impl_no_neg_occ; wf_auto2.
+      * apply fresh_svar_no_neg. unfold svar_is_fresh_in.
+        subst X.
+        pose proof free_svars_free_evar_subst.
+        eapply not_elem_of_larger_impl_not_elem_of;
+  [|apply X_eq_fresh_impl_X_notin_free_svars; reflexivity];
+      cbn; set_solver.
+    }
+    {
+      apply svar_hno_bsvar_subst.
+      * intros. cbn in H2. congruence.
+      * intros. clear-H WF1 WF2. wf_auto2.
+        all: try apply wfc_impl_no_pos_occ; try apply wfc_impl_no_neg_occ; wf_auto2.
+      * apply fresh_svar_no_neg. unfold svar_is_fresh_in.
+        subst X.
+        pose proof free_svars_free_evar_subst.
+        eapply not_elem_of_larger_impl_not_elem_of;
+  [|apply X_eq_fresh_impl_X_notin_free_svars; reflexivity];
+      cbn; set_solver.
+    }
+    mlSimpl.
+    rewrite svar_open_not_occur. wf_auto2.
+    rewrite svar_open_not_occur. wf_auto2.
+    unfold svar_open.
+    rewrite -free_evar_subst_bsvar_subst. wf_auto2. unfold evar_is_fresh_in; set_solver.
+    rewrite -free_evar_subst_bsvar_subst. wf_auto2. unfold evar_is_fresh_in; set_solver.
+    mlIntro. mlDestructAnd "0".
+    fromMLGoal.
+    apply IHsz.
+    - assumption.
+    - rewrite svar_open_size'. lia.
+    - wf_auto2.
+    - wf_auto2.
+    - wf_auto2.
+    - destruct_and!.
+      apply kt_well_formed_svar_open; wf_auto2.
+Defined.
 
 
 Local Lemma simplTest
